Utils.thy
@@ -1,0 +1,209 @@
+
+theory Utils
+  imports Main
+begin
+
+
+text \<open>The following functions transform a list L to a relation containing a  tuple $(a,b)$
+  iff $a = b$ or $a$ precedes $b$ in the list L \<close>
+
+fun list_to_rel:: "'a list \<Rightarrow> 'a rel"
+  where "list_to_rel [] = {}"
+  | "list_to_rel (x#xs) = {x} \<times> (set (x#xs)) \<union> list_to_rel xs"
+
+
+lemma list_to_rel_in : " (a,b)  \<in> (list_to_rel L) \<longrightarrow> a \<in> set L \<and> b \<in> set L" 
+proof(induct L, auto) qed
+
+text \<open>Show soundness of list-to-rel\<close>
+lemma list_to_rel_equal: 
+"(a,b) \<in> list_to_rel L \<longleftrightarrow> (\<exists>k::nat. hd (drop k L) = a \<and> b \<in> set (drop k L))"
+proof(safe)
+  assume "(a, b) \<in> list_to_rel L"
+  then show "\<exists>k. hd (drop k L) = a \<and> b \<in> set  (drop k L)"
+  proof(induct L)
+    case Nil
+    then show ?case by auto
+  next
+    case (Cons a2 L)
+    then consider "(a, b) \<in> {a2} \<times> set (a2 # L) " | "(a,b) \<in>  list_to_rel L" by auto
+    then show ?case unfolding list_to_rel.simps(2)  
+    proof(cases)
+      case 1
+      then have "a = hd (a2 # L)" by auto
+      moreover have "b \<in> set (a2 # L)" using 1 by auto
+      ultimately show ?thesis using drop0
+        by metis 
+    next
+      case 2
+      then obtain k where k_in : "hd (drop k (L)) = a \<and> b \<in> set (drop k (L))" 
+        using Cons(1) by auto
+      show ?thesis proof
+        let ?k = "Suc k"
+        show "hd (drop ?k (a2 # L)) = a \<and> b \<in> set (drop ?k (a2 # L))"
+          unfolding drop_Suc using k_in by auto 
+      qed
+  qed
+    qed
+  next
+  fix k 
+  assume "b \<in> set (drop k L)"
+  and "a = hd (drop k L)"
+  then show "(hd (drop k L), b) \<in> list_to_rel L"
+  proof(induct L arbitrary: k)
+    case Nil
+    then show ?case by auto
+  next
+    case (Cons a L)
+    consider (zero) "k = 0" | (more) "k > 0" by auto    
+    then show ?case 
+    proof(cases)
+      case zero
+    then show ?thesis using Cons drop_0 by auto
+  next
+    case more
+    then obtain k2 where k2_in:  "k = Suc k2"
+      using gr0_implies_Suc by auto 
+     show ?thesis using Cons unfolding k2_in drop_Suc list_to_rel.simps(2) by auto
+    qed
+  qed
+qed
+
+lemma list_to_rel_append:
+  assumes "a \<in> set L"
+  shows "(a,b) \<in> list_to_rel (L @ [b])" 
+  using assms
+proof(induct L, simp, auto) qed 
+
+text \<open>For every distinct L, list-to-rel L return a linear order on set L\<close>
+lemma list_order_linear:
+  assumes "distinct L"
+  shows "linear_order_on (set L)  (list_to_rel L)" 
+  unfolding linear_order_on_def total_on_def partial_order_on_def preorder_on_def refl_on_def
+  trans_def antisym_def 
+proof(safe)
+  fix a b
+  assume "(a, b) \<in> list_to_rel L"
+  then show "a \<in> set L" 
+  proof(induct L, auto) qed
+next 
+  fix a b
+  assume "(a, b) \<in> list_to_rel L"
+  then show "b \<in> set L" 
+  proof(induct L, auto) qed
+next 
+  fix x 
+  assume "x \<in> set L"
+  then show "(x, x) \<in> list_to_rel L"
+  proof(induct L, auto) qed
+next
+  fix x y z 
+  assume as1: "(x,y) \<in> list_to_rel L"
+  and  as2: "(y, z) \<in> list_to_rel L"
+  then show "(x, z) \<in> list_to_rel L"
+    using assms
+  proof(induct L)
+    case Nil
+    then show ?case by auto
+  next
+    case (Cons a L)
+    then consider (nor) "(x, y) \<in> {a} \<times> set (a # L) \<and> (y, z) \<in> {a} \<times> set (a # L)" 
+      | (xy) "(x,y) \<in> list_to_rel L \<and> (y, z) \<in> {a} \<times> set (a # L)" 
+      | (yz) "(y,z) \<in> list_to_rel L \<and> (x, y) \<in> {a} \<times> set (a # L)"
+      | (both) "(y,z) \<in> list_to_rel L \<and> (x,y) \<in> list_to_rel L" by auto
+    then show ?case proof(cases)
+    case nor
+      then show ?thesis by auto
+    next
+      case xy 
+      then have "y \<in> set L" using list_to_rel_in by metis
+      also have "y = a" using xy by auto
+      ultimately have "\<not> distinct (a # L)"
+        by simp 
+    then show ?thesis using Cons by auto
+    next
+    case yz
+    then show ?thesis using list_to_rel.simps(2)
+      by (metis Cons.prems(2) SigmaD1 SigmaI UnI1 list_to_rel_in)  
+    next
+      case both
+      then show ?thesis unfolding list_to_rel.simps(2) using Cons by auto
+    qed
+  qed 
+next
+  fix x y 
+  assume "(x, y) \<in> list_to_rel L"
+  and "(y, x) \<in> list_to_rel L"
+  then show "x = y"
+    using assms
+  proof(induct L, simp)
+    case (Cons a L)
+      then consider (nor) "(x, y) \<in> {a} \<times> set (a # L) \<and> (y, x) \<in> {a} \<times> set (a # L)" 
+      | (xy) "(x,y) \<in> list_to_rel L \<and> (y, x) \<in> {a} \<times> set (a # L)" 
+      | (yz) "(y,x) \<in> list_to_rel L \<and> (x, y) \<in> {a} \<times> set (a # L)"
+      | (both) "(y,x) \<in> list_to_rel L \<and> (x,y) \<in> list_to_rel L" by auto
+      then show ?case unfolding list_to_rel.simps 
+      proof(cases)
+      case nor
+      then show ?thesis by auto
+      next
+      case xy
+      then show ?thesis
+        by (metis Cons.prems(3) SigmaD1 distinct.simps(2) list_to_rel_in singletonD) 
+      next
+        case yz
+        then show ?thesis  
+          by (metis Cons.prems(3) SigmaD1 distinct.simps(2) list_to_rel_in singletonD) 
+      next
+        case both
+      then show ?thesis using Cons by auto 
+      qed
+    qed
+  next
+    fix x y 
+    assume "x \<in> set L"
+    and "y \<in> set L"
+    and "x \<noteq> y"
+    and "(y, x) \<notin> list_to_rel L"
+    then show "(x, y) \<in> list_to_rel L"
+    proof(induct L, auto) qed    
+  qed
+
+
+lemma list_to_rel_mono:
+  assumes "(a,b) \<in> list_to_rel (L)"
+  shows "(a,b) \<in> list_to_rel (L @ L2)"
+  using assms
+proof(induct L2 arbitrary: L, simp)
+  case (Cons a L2)
+  then show ?case 
+  proof(induct L, auto)
+  qed
+qed
+
+lemma list_to_rel_mono2:
+  assumes "(a,b) \<in> list_to_rel (L2)"
+  shows "(a,b) \<in> list_to_rel (L @ L2)"
+  using assms
+proof(induct L2 arbitrary: L, simp)
+  case (Cons a L2)
+  then show ?case 
+  proof(induct L, auto)
+  qed
+qed
+
+
+
+lemma map_snd_map: "\<And>L. (map snd (map (\<lambda>i. (P i , i)) L)) =  L" 
+proof -
+  fix L
+  show "map snd (map (\<lambda>i. (P i, i)) L) = L"
+  proof(induct L)
+    case Nil
+    then show ?case by auto
+  next
+    case (Cons a L)
+    then show ?case by auto
+  qed
+qed
+end
