ROOT
@@ -2,6 +2,9 @@ session Isabelle = HOL +
   options [document = pdf, document_output = "output"]
   sessions "Graph_Theory"
   theories
+	Utils
+	DigraphUtils
+	TopSort
 	blockDAG
     Spectre
 	Ghostdag
